store/server_proofs/create.v
@@ -1,0 +1,143 @@
+From stdpp Require Import base gmap.
+From mathcomp Require Import ssreflect.
+From stdpp Require Import namespaces.
+From iris.algebra Require Import agree auth csum gset gmap excl frac.
+From iris.algebra Require Import max_prefix_list.
+From iris.heap_lang Require Import notation proofmode.
+From cryptis Require Import lib version term cryptis primitives tactics.
+From cryptis Require Import role session pk_auth pk_dh.
+From cryptis.store Require Import impl shared alist db.
+
+Set Implicit Arguments.
+Unset Strict Implicit.
+Unset Printing Implicit Defensive.
+
+Section Verif.
+
+Context `{!cryptisGS Σ, !heapGS Σ, !sessionGS Σ}.
+Notation iProp := (iProp Σ).
+
+Context `{!storeGS Σ}.
+
+Local Instance STORE : PK := PK_DH (λ _ _ _ _, True)%I.
+
+Implicit Types (cs : cst) (ss : sst).
+Implicit Types kI kR kS t : term.
+Implicit Types n : nat.
+Implicit Types γ : gname.
+Implicit Types v : val.
+
+Variable N : namespace.
+
+Lemma wp_server_handle_create E c ss m :
+  ↑cryptisN ⊆ E →
+  channel c -∗
+  store_ctx N -∗
+  public m -∗
+  {{{ server N ss }}}
+    Server.handle_create N c (repr ss) m @ E
+  {{{ (v : option val), RET (repr v); server N ss }}}.
+Proof.
+iIntros "%sub #chan_c #ctx #p_m !> %Φ state post".
+rewrite /Server.handle_create. wp_pures.
+iDestruct "state" as "(%n & %kvs & %db & #handshake & #minted_key & ts &
+                       db & %kvs_db & #pub_db & #view)".
+wp_load. wp_pures. wp_load. wp_pures.
+iAssert (server N ss) with "[ts db view]" as "state".
+{ iExists n, kvs, db. iFrame. eauto. }
+wp_tsdec m; wp_pures; last by iApply ("post" $! None).
+wp_list_of_term m; wp_pures; last by iApply ("post" $! None).
+wp_list_match => [timestamp t1 t2 ->| _]; wp_pures; last by iApply ("post" $! None).
+wp_bind (to_int _). iApply wp_to_int.
+case: Spec.to_intP => [ {m} n' ->| _]; wp_pures;
+  last by iApply ("post" $! None).
+case: bool_decide_reflect => [[<-] {n'}|?]; wp_pures;
+  last by iApply ("post" $! None).
+wp_bind (AList.find _ _). iApply AList.wp_find => //.
+iIntros "!> _".
+iDestruct "ctx" as "(_ & _ & _ & _ & _ & ? & ? & _)".
+wp_bind (match: _ with InjL <> => _ | InjR <> => _ end)%E.
+iApply (wp_wand _ _ _ (λ v, server N ss ∗ ∃ b : bool,
+  ⌜v = #(((if b then 1 else 0) : Z))⌝ ∗
+  (⌜b = false⌝ ∨
+   ⌜b = true⌝ ∗
+   if sst_ok ss then
+     ∃ γ, wf_key N (sst_key ss) γ ∗ DB.free_at γ n t1
+   else True))%I with "[state]").
+{ case db_t1: (db !! t1) => [t2'|]; wp_pures;
+    first by iFrame; iExists false; eauto.
+  iDestruct "state" as "(%n' & %kvs' & %db' & _ & _ & ts & db & _ & _ & _)".
+  wp_bind (AList.insert _ _ _). iApply AList.wp_insert => //.
+  iIntros "!> %kvs'' %kvs''_db'". wp_store. wp_pures.
+  iDestruct (public_TEncE with "p_m [//]") as "{p_m} [p_m|p_m]".
+  - case is_ok: sst_ok.
+    { iDestruct "view" as "(%γ & (#contra & _) & _)".
+      iDestruct "p_m" as "[p_k _]".
+      iDestruct ("contra" with "p_k") as ">[]". }
+    wp_store.
+    have -> : (n + 1)%Z = S n :> Z by lia.
+    iModIntro. iSplit; last by iExists true; eauto.
+    iExists (S n), kvs'', _. iFrame. rewrite is_ok.
+    do 4!iSplit => //.
+    iApply big_sepM_insert_2 => //.
+    rewrite public_of_list /=.
+    by iDestruct "p_m" as "(_ & _ & ? & ? & _)"; eauto.
+  - iDestruct "p_m" as "(#p_m & _)". wp_store.
+    have -> : (n + 1)%Z = S n :> Z by lia.
+    iDestruct "p_m" as "(%γ & %n'' & %t1' & %t2' & %ok & %e & handshake' &
+                         wf & p_t1 & p_t2 & t1_t2)".
+    case/Spec.of_list_inj: e => e <- <- {t1' t2'}.
+    have {n'' e} <- : n = n'' by lia.
+    case is_ok: sst_ok => //; last first.
+    { iSplitL; last by iExists true; eauto.
+      iModIntro. iExists (S n), kvs'', _. iFrame. rewrite is_ok.
+      do 4!iSplit => //.
+      iApply big_sepM_insert_2 => //.
+      by eauto. }
+    iDestruct "view" as "(%γ' & wf' & view)".
+    iPoseProof (handshake_done_agree with "wf' handshake handshake'")
+      as "<-".
+    iPoseProof (wf_key_agree with "handshake wf' wf") as "->".
+    iSplitL.
+    + iModIntro.
+      iExists (S n), kvs'', _. iFrame. rewrite is_ok.
+      do 4!iSplit => //.
+      * iApply big_sepM_insert_2 => //.
+        by eauto.
+      * iExists γ. iSplit => //. by iApply DB.create_server.
+    + iExists true. iSplitR => //.
+      iRight. iSplitR => //. iExists γ. iModIntro. iSplit => //.
+      by iApply DB.free_atI. }
+iIntros "%v (state & %b & -> & #vP)".
+wp_pures. wp_bind (tint _). iApply wp_tint. wp_list.
+wp_bind (tint _). iApply wp_tint. wp_list. wp_term_of_list.
+iAssert (▷ (public t1 ∗ public t2))%I as "[p_t1 p_t2]".
+  { iDestruct (public_TEncE with "p_m [//]") as "{p_m} [[_ p_m]|p_m]".
+    - rewrite public_of_list /=. iDestruct "p_m" as "(_ & ? & ? & _)".
+      by eauto.
+    - iDestruct "p_m" as "(#p_m & _)". iModIntro.
+      iDestruct "p_m" as "(%γ & %n'' & %t1' & %t2' & %ok & %e &
+                           _ & ? & ? & ? & _)".
+      by case/Spec.of_list_inj: e => _ <- <-; eauto. }
+wp_pures. wp_tsenc. wp_bind (send _ _).
+iApply (wp_send with "[//] [#]") => //; last by wp_pures;
+  iApply ("post" $! (Some #())).
+iModIntro. iApply public_TEncIS => //.
+- rewrite minted_TKey.
+  iPoseProof (public_minted with "p_m") as "{p_m} p_m".
+  by rewrite minted_TEnc; iDestruct "p_m" as "[??]".
+- iModIntro. iExists n, t1, t2, b, (sst_ok ss). iSplit => //.
+  iSplit => //.
+  case: sst_ok => //.
+  iDestruct "view" as "(%γ & key & view)".
+  iExists γ. iSplit => //.
+  iDestruct "vP" as "[->| (-> & vP)]" => //.
+  iDestruct "vP" as "(%γ' & key' & free)".
+  by iPoseProof (wf_key_agree with "handshake key key'") as "->".
+- iPoseProof (public_minted with "p_m") as "m_m".
+  rewrite minted_TEnc minted_tag !minted_of_list /= !minted_TInt.
+  iDestruct "m_m" as "(? & _ & ? & ? & _)". by eauto.
+- iIntros "!> _". by rewrite public_of_list /= !public_TInt; eauto.
+Qed.
+
+End Verif.
