store/server_proofs/load.v
@@ -1,0 +1,78 @@
+From stdpp Require Import base gmap.
+From mathcomp Require Import ssreflect.
+From stdpp Require Import namespaces.
+From iris.algebra Require Import agree auth csum gset gmap excl frac.
+From iris.algebra Require Import max_prefix_list.
+From iris.heap_lang Require Import notation proofmode.
+From cryptis Require Import lib version term cryptis primitives tactics.
+From cryptis Require Import role session pk_auth pk_dh.
+From cryptis.store Require Import impl shared alist db.
+
+Set Implicit Arguments.
+Unset Strict Implicit.
+Unset Printing Implicit Defensive.
+
+Section Verif.
+
+Context `{!cryptisGS Σ, !heapGS Σ, !sessionGS Σ}.
+Notation iProp := (iProp Σ).
+
+Context `{!storeGS Σ}.
+
+Local Instance STORE : PK := PK_DH (λ _ _ _ _, True)%I.
+
+Implicit Types (cs : cst) (ss : sst).
+Implicit Types kI kR kS t : term.
+Implicit Types n : nat.
+Implicit Types γ : gname.
+Implicit Types v : val.
+
+Variable N : namespace.
+
+Lemma wp_server_handle_load E c ss m :
+  ↑cryptisN ⊆ E →
+  channel c -∗
+  store_ctx N -∗
+  public m -∗
+  {{{ server N ss }}}
+    Server.handle_load N c (repr ss) m @ E
+  {{{ (v : option val), RET (repr v); server N ss }}}.
+Proof.
+iIntros "%sub #chan_c #ctx #p_m !> %Φ state post".
+rewrite /Server.handle_load. wp_pures.
+iDestruct "state" as "(%n & %kvs & %db & #handshake & #minted_key & ts &
+                       db & %kvs_db & #pub_db & #view)".
+wp_load. wp_pures. wp_load. wp_pures.
+iAssert (server N ss) with "[ts db view]" as "state".
+{ iExists n, kvs, db. iFrame. eauto. }
+wp_tsdec m; wp_pures; last by iApply ("post" $! None).
+wp_list_of_term m; wp_pures; last by iApply ("post" $! None).
+wp_list_match => [timestamp t1 ->| _]; wp_pures; last by iApply ("post" $! None).
+wp_bind (to_int _). iApply wp_to_int.
+case: Spec.to_intP => [ {m} n' -> | _]; wp_pures; last by iApply ("post" $! None).
+case: bool_decide_reflect => [[<-]|?]; wp_pures; last by iApply ("post" $! None).
+wp_bind (AList.find _ _). iApply AList.wp_find => //.
+iIntros "!> _".
+case db_t1: (db !! t1) => [t2|]; wp_pures; last by iApply ("post" $! None).
+wp_list. wp_bind (tint _). iApply wp_tint. wp_list. wp_term_of_list.
+wp_pures. wp_tsenc. wp_bind (send _ _).
+iApply (wp_send with "[//] [#]") => //; last by wp_pures;
+  iApply ("post" $! (Some #())).
+iDestruct "ctx" as "(_ & _ & _ & _ & ? & _)".
+iModIntro.
+rewrite big_sepM_delete //. iDestruct "pub_db" as "[[? ?] _]".
+iApply public_TEncIS => //.
+- rewrite minted_TKey.
+  iPoseProof (public_minted with "p_m") as "{p_m} p_m".
+  by rewrite minted_TEnc; iDestruct "p_m" as "[??]".
+- iModIntro. iExists n, (sst_ok ss), t1, t2. iSplit => //.
+  do 2!iSplit => //.
+  case: sst_ok => //.
+  iDestruct "view" as "(%γ & key & view)".
+  iExists γ. iSplit => //. iApply DB.load_server; eauto.
+- rewrite minted_of_list /= minted_TInt -[minted t1]public_minted.
+  rewrite -[minted t2]public_minted; eauto.
+- iIntros "!> _". by rewrite public_of_list /= public_TInt; eauto.
+Qed.
+
+End Verif.
