store/server_proofs/store.v
@@ -1,0 +1,91 @@
+From stdpp Require Import base gmap.
+From mathcomp Require Import ssreflect.
+From stdpp Require Import namespaces.
+From iris.algebra Require Import agree auth csum gset gmap excl frac.
+From iris.algebra Require Import max_prefix_list.
+From iris.heap_lang Require Import notation proofmode.
+From cryptis Require Import lib version term cryptis primitives tactics.
+From cryptis Require Import role session pk_auth pk_dh.
+From cryptis.store Require Import impl shared alist db.
+
+Set Implicit Arguments.
+Unset Strict Implicit.
+Unset Printing Implicit Defensive.
+
+Section Verif.
+
+Context `{!cryptisGS Σ, !heapGS Σ, !sessionGS Σ}.
+Notation iProp := (iProp Σ).
+
+Context `{!storeGS Σ}.
+
+Local Instance STORE : PK := PK_DH (λ _ _ _ _, True)%I.
+
+Implicit Types (cs : cst) (ss : sst).
+Implicit Types kI kR kS t : term.
+Implicit Types n : nat.
+Implicit Types γ : gname.
+Implicit Types v : val.
+
+Variable N : namespace.
+
+Lemma ack_storeI kS n :
+  store_ctx N -∗
+  minted kS -∗
+  public (TEnc kS (Spec.tag (N.@"ack_store") (TInt n))).
+Proof.
+iIntros "(_ & _ & #ctx & _) #s_kS".
+iApply public_TEncIS => //.
+- by rewrite minted_TKey.
+- iModIntro. by iExists n.
+- by rewrite minted_TInt.
+- by rewrite public_TInt; eauto.
+Qed.
+
+Lemma wp_server_handle_store E c ss m :
+  ↑cryptisN ⊆ E →
+  channel c -∗
+  store_ctx N -∗
+  public m -∗
+  {{{ server N ss }}}
+    Server.handle_store N c (repr ss) m @ E
+  {{{ (v : option val), RET (repr v); server N ss }}}.
+Proof.
+iIntros "%sub #chan_c #ctx #p_m !> %Φ state post".
+rewrite /Server.handle_store. wp_pures.
+wp_tsdec m; wp_pures; last by iApply ("post" $! None).
+wp_list_of_term m; wp_pures; last by iApply ("post" $! None).
+wp_list_match => [n' t1 t2 ->|_]; wp_pures; last by iApply ("post" $! None).
+wp_bind (to_int _). iApply wp_to_int.
+case: Spec.to_intP => [ {}n' -> | _]; wp_pures; last by iApply ("post" $! None).
+iDestruct "state" as "(%n & %kvs & %db & #handshake & #minted_key & ts &
+                       db & %kvs_db & #pub_db & view)".
+wp_load. wp_pures.
+case: bool_decide_reflect => [[<-]|ne]; wp_pures; last first.
+{ iModIntro. iApply ("post" $! None).
+  iExists n, kvs, db. iFrame. by eauto. }
+wp_load. wp_pures.
+replace (n + 1)%Z with (S n : Z) by lia.
+wp_store. wp_load. wp_bind (AList.insert _ _ _).
+wp_pures. iApply AList.wp_insert; eauto. iIntros "!> %kvs' %kvs'_db'".
+iDestruct (store_predE with "handshake [#] [//] p_m") as "(p_t1 & p_t2 & wf')".
+{ case: sst_ok => //.
+  iDestruct "view" as "(%γ & ? & ?)". eauto. }
+wp_store. wp_bind (tint _). iApply wp_tint.
+wp_tsenc.
+iApply wp_fupd.
+wp_bind (send _ _). iApply wp_send => //.
+{ iModIntro. iApply ack_storeI => //. }
+wp_pures. iApply ("post" $! (Some #())).
+iExists (S n), kvs', (<[t1 := t2]>db). iFrame.
+do 4!iSplitR => //.
+{ iModIntro. iApply big_sepM_insert_2 => //. eauto. }
+case: sst_ok; eauto.
+iDestruct "wf'" as "(%γ1 & wf1 & update)".
+iDestruct "view" as "(%γ2 & #wf2 & #view)".
+iPoseProof (wf_key_agree with "handshake wf1 wf2") as "<-".
+iPoseProof (DB.update_server with "view update") as "view'".
+iModIntro. iExists γ1. iSplit => //.
+Qed.
+
+End Verif.
